downstream: update repo cslib
downstream-repo: cslib
downstream-url: https://github.com/leanprover/cslib
downstream-rev: main
downstream-sha: c2197aca422e341b78650acb69b5441b30139d21

cslib/Cslib/Foundations/Semantics/LTS/Basic.lean
@@ -170,6 +170,22 @@ theorem MTr.append_iff : lts.MTr s1 (μs ++ μs') s2 ↔ ∃ s, lts.MTr s1 μs s
   intro ⟨_, h, h'⟩
   exact h.comp lts h'
 
+/-- Single-step invariant. -/
+@[scoped grind =]
+def TrInv (p : State → Prop) : Prop :=
+  ∀ s1 μ s2, lts.Tr s1 μ s2 → p s1 → p s2
+
+/-- Multistep invariant. -/
+@[scoped grind =]
+def MTrInv (p : State → Prop) : Prop :=
+  ∀ s1 μs s2, lts.MTr s1 μs s2 → p s1 → p s2
+
+/-- Any single-step invariant is also a multistep invariant. -/
+theorem mtrInv_of_trInv {lts : LTS State Label} {p : State → Prop}
+    (htr : lts.TrInv p) : lts.MTrInv p := by
+  intro s1 μs s2 h
+  induction h <;> grind
+
 /-- A state `s1` can reach a state `s2` if there exists a multistep transition from
 `s1` to `s2`. -/
 @[scoped grind =]
